formal/fstar/ocaml-output/Parser_NQuads.ml
@@ -1,5 +1,5 @@
 open Prims
-let parse_graph_label : RDF_Graph_Executable.iri Parser_Combinators.parser=
+let parse_graph_label : RDF_Term.iri Parser_Combinators.parser=
   fun input pos ->
     let len = Parser_FastString.fs_byte_length input in
     if pos >= len
@@ -11,7 +11,7 @@ let parse_graph_label : RDF_Graph_Executable.iri Parser_Combinators.parser=
        then
          match Parser_NTriples.parse_iri_raw input pos with
          | Parser_Combinators.ParseOk (iri, pos') ->
-             (if RDF_Graph_Executable.is_iri iri
+             (if RDF_Term.is_iri iri
               then Parser_Combinators.ParseOk (iri, pos')
               else
                 Parser_Combinators.ParseFail
@@ -31,8 +31,7 @@ let parse_graph_label : RDF_Graph_Executable.iri Parser_Combinators.parser=
            Parser_Combinators.ParseFail
              ("expected '<' or '_:' for graph label", pos))
 let parse_opt_graph_label :
-  RDF_Graph_Executable.iri FStar_Pervasives_Native.option
-    Parser_Combinators.parser=
+  RDF_Term.iri FStar_Pervasives_Native.option Parser_Combinators.parser=
   fun input pos ->
     let len = Parser_FastString.fs_byte_length input in
     match Parser_NTriples.pws input pos with
@@ -68,8 +67,8 @@ let parse_opt_graph_label :
     | Parser_Combinators.ParseFail (msg, fpos) ->
         Parser_Combinators.ParseFail (msg, fpos)
 let parse_nquad :
-  (RDF_Graph_Executable.triple * RDF_Graph_Executable.iri
-    FStar_Pervasives_Native.option) Parser_Combinators.parser=
+  (RDF_Triple.triple * RDF_Term.iri FStar_Pervasives_Native.option)
+    Parser_Combinators.parser=
   fun input pos ->
     match Parser_NTriples.pws input pos with
     | Parser_Combinators.ParseOk ((), pos1) ->
@@ -106,18 +105,13 @@ let parse_nquad :
                                                 (FStar_Char.int_of_char dot)
                                                   = (Prims.of_int (0x2E))
                                               then
-                                                (if
-                                                   RDF_Graph_Executable.is_iri
-                                                     pred
+                                                (if RDF_Term.is_iri pred
                                                  then
                                                    let t =
                                                      {
-                                                       RDF_Graph_Executable.s
-                                                         = subj;
-                                                       RDF_Graph_Executable.p
-                                                         = pred;
-                                                       RDF_Graph_Executable.o
-                                                         = obj
+                                                       RDF_Triple.s = subj;
+                                                       RDF_Triple.p = pred;
+                                                       RDF_Triple.o = obj
                                                      } in
                                                    Parser_Combinators.ParseOk
                                                      ((t, graph_opt),
@@ -149,68 +143,53 @@ let parse_nquad :
              Parser_Combinators.ParseFail (msg, fpos))
     | Parser_Combinators.ParseFail (msg, fpos) ->
         Parser_Combinators.ParseFail (msg, fpos)
-let rec find_named_graph (name : RDF_Graph_Executable.iri)
-  (ngs : RDF_Graph_Executable.named_graph Prims.list) :
-  (RDF_Graph_Executable.named_graph Prims.list *
-    RDF_Graph_Executable.rdf_graph * RDF_Graph_Executable.named_graph
-    Prims.list) FStar_Pervasives_Native.option=
+let rec find_named_graph (name : RDF_Term.iri)
+  (ngs : RDF_Graph.named_graph Prims.list) :
+  (RDF_Graph.named_graph Prims.list * RDF_Graph.rdf_graph *
+    RDF_Graph.named_graph Prims.list) FStar_Pervasives_Native.option=
   match ngs with
   | [] -> FStar_Pervasives_Native.None
   | ng::rest ->
-      if ng.RDF_Graph_Executable.ng_name = name
-      then
-        FStar_Pervasives_Native.Some
-          ([], (ng.RDF_Graph_Executable.ng_graph), rest)
+      if ng.RDF_Graph.ng_name = name
+      then FStar_Pervasives_Native.Some ([], (ng.RDF_Graph.ng_graph), rest)
       else
         (match find_named_graph name rest with
          | FStar_Pervasives_Native.Some (before, g, after) ->
              FStar_Pervasives_Native.Some ((ng :: before), g, after)
          | FStar_Pervasives_Native.None -> FStar_Pervasives_Native.None)
-let dataset_add_quad (ds : RDF_Graph_Executable.rdf_dataset)
-  (t : RDF_Graph_Executable.triple)
-  (graph_name : RDF_Graph_Executable.iri FStar_Pervasives_Native.option) :
-  RDF_Graph_Executable.rdf_dataset=
+let dataset_add_quad (ds : RDF_Graph.rdf_dataset) (t : RDF_Triple.triple)
+  (graph_name : RDF_Term.iri FStar_Pervasives_Native.option) :
+  RDF_Graph.rdf_dataset=
   match graph_name with
   | FStar_Pervasives_Native.None ->
       {
-        RDF_Graph_Executable.ds_default =
-          (RDF_Graph_Executable.graph_add_unchecked t
-             ds.RDF_Graph_Executable.ds_default);
-        RDF_Graph_Executable.ds_named = (ds.RDF_Graph_Executable.ds_named)
+        RDF_Graph.ds_default =
+          (RDF_Graph_Executable.graph_add_unchecked t ds.RDF_Graph.ds_default);
+        RDF_Graph.ds_named = (ds.RDF_Graph.ds_named)
       }
   | FStar_Pervasives_Native.Some name ->
-      (match find_named_graph name ds.RDF_Graph_Executable.ds_named with
+      (match find_named_graph name ds.RDF_Graph.ds_named with
        | FStar_Pervasives_Native.Some (before, existing_g, after) ->
            let updated_g =
              RDF_Graph_Executable.graph_add_unchecked t existing_g in
            let updated_ng =
-             {
-               RDF_Graph_Executable.ng_name = name;
-               RDF_Graph_Executable.ng_graph = updated_g
-             } in
+             { RDF_Graph.ng_name = name; RDF_Graph.ng_graph = updated_g } in
            {
-             RDF_Graph_Executable.ds_default =
-               (ds.RDF_Graph_Executable.ds_default);
-             RDF_Graph_Executable.ds_named =
+             RDF_Graph.ds_default = (ds.RDF_Graph.ds_default);
+             RDF_Graph.ds_named =
                (FStar_List_Tot_Base.op_At before
                   (FStar_List_Tot_Base.op_At [updated_ng] after))
            }
        | FStar_Pervasives_Native.None ->
            let new_ng =
-             {
-               RDF_Graph_Executable.ng_name = name;
-               RDF_Graph_Executable.ng_graph = [t]
-             } in
+             { RDF_Graph.ng_name = name; RDF_Graph.ng_graph = [t] } in
            {
-             RDF_Graph_Executable.ds_default =
-               (ds.RDF_Graph_Executable.ds_default);
-             RDF_Graph_Executable.ds_named =
-               (FStar_List_Tot_Base.op_At ds.RDF_Graph_Executable.ds_named
-                  [new_ng])
+             RDF_Graph.ds_default = (ds.RDF_Graph.ds_default);
+             RDF_Graph.ds_named =
+               (FStar_List_Tot_Base.op_At ds.RDF_Graph.ds_named [new_ng])
            })
 let rec parse_nquads_acc (input : Prims.string) (pos : Prims.nat)
-  (ds : RDF_Graph_Executable.rdf_dataset) (fuel : Prims.nat) :
-  RDF_Graph_Executable.rdf_dataset=
+  (ds : RDF_Graph.rdf_dataset) (fuel : Prims.nat) : RDF_Graph.rdf_dataset=
   if fuel = Prims.int_zero
   then ds
   else
@@ -281,11 +260,109 @@ let rec parse_nquads_acc (input : Prims.string) (pos : Prims.nat)
                     then ds
                     else
                       parse_nquads_acc input pos2 ds (fuel - Prims.int_one)))))
-let parse_nquads (input : Prims.string) : RDF_Graph_Executable.rdf_dataset=
+let parse_nquads (input : Prims.string) : RDF_Graph.rdf_dataset=
   let len = Parser_FastString.fs_byte_length input in
   RDF_Graph_Executable.dataset_finalise
-    (parse_nquads_acc input Prims.int_zero RDF_Graph_Executable.empty_dataset
+    (parse_nquads_acc input Prims.int_zero RDF_Graph.empty_dataset
        (len + Prims.int_one))
+let rec fold_nquads_acc :
+  'a .
+    (RDF_Triple.triple ->
+       RDF_Term.iri FStar_Pervasives_Native.option -> 'a -> 'a)
+      ->
+      ('a -> Prims.bool) ->
+        Prims.string -> Prims.nat -> 'a -> Prims.nat -> 'a
+  =
+  fun step stop input pos acc fuel ->
+    if fuel = Prims.int_zero
+    then acc
+    else
+      if stop acc
+      then acc
+      else
+        (let len = Parser_FastString.fs_byte_length input in
+         if pos >= len
+         then acc
+         else
+           (let pos1 =
+              match Parser_NTriples.pws input pos with
+              | Parser_Combinators.ParseOk ((), p) -> p
+              | uu___3 -> pos in
+            if pos1 >= len
+            then acc
+            else
+              (let ch = Parser_FastString.fs_byte_index input pos1 in
+               let code = FStar_Char.int_of_char ch in
+               if code = (Prims.of_int (0x23))
+               then
+                 let pos2 = Parser_NTriples.skip_comment input pos1 in
+                 let pos3 = Parser_NTriples.skip_eol input pos2 in
+                 (if pos3 = pos1
+                  then acc
+                  else
+                    fold_nquads_acc step stop input pos3 acc
+                      (fuel - Prims.int_one))
+               else
+                 if
+                   (code = (Prims.of_int (0x0A))) ||
+                     (code = (Prims.of_int (0x0D)))
+                 then
+                   (let pos2 = Parser_NTriples.skip_eol input pos1 in
+                    if pos2 = pos1
+                    then acc
+                    else
+                      fold_nquads_acc step stop input pos2 acc
+                        (fuel - Prims.int_one))
+                 else
+                   (match parse_nquad input pos1 with
+                    | Parser_Combinators.ParseOk ((t, graph_opt), pos2) ->
+                        let acc1 = step t graph_opt acc in
+                        let pos3 =
+                          match Parser_NTriples.pws input pos2 with
+                          | Parser_Combinators.ParseOk ((), p) -> p
+                          | uu___6 -> pos2 in
+                        let pos4 = Parser_NTriples.skip_comment input pos3 in
+                        let pos5 = Parser_NTriples.skip_eol input pos4 in
+                        let pos_next =
+                          if pos5 > pos1
+                          then pos5
+                          else if pos4 > pos1 then pos4 else pos2 in
+                        if stop acc1
+                        then acc1
+                        else
+                          fold_nquads_acc step stop input pos_next acc1
+                            (fuel - Prims.int_one)
+                    | Parser_Combinators.ParseFail (uu___6, uu___7) ->
+                        let rec skip_line p f =
+                          if f = Prims.int_zero
+                          then p
+                          else
+                            if p >= len
+                            then p
+                            else
+                              (let c =
+                                 Parser_FastString.fs_byte_index input p in
+                               let cc = FStar_Char.int_of_char c in
+                               if
+                                 (cc = (Prims.of_int (0x0A))) ||
+                                   (cc = (Prims.of_int (0x0D)))
+                               then Parser_NTriples.skip_eol input p
+                               else
+                                 skip_line (p + Prims.int_one)
+                                   (f - Prims.int_one)) in
+                        let pos2 = skip_line pos1 (len - pos1) in
+                        if pos2 = pos1
+                        then acc
+                        else
+                          fold_nquads_acc step stop input pos2 acc
+                            (fuel - Prims.int_one)))))
+let fold_nquads
+  (step :
+    RDF_Triple.triple ->
+      RDF_Term.iri FStar_Pervasives_Native.option -> 'a -> 'a)
+  (stop : 'a -> Prims.bool) (init : 'a) (input : Prims.string) : 'a=
+  let len = Parser_FastString.fs_byte_length input in
+  fold_nquads_acc step stop input Prims.int_zero init (len + Prims.int_one)
 let validate_graph_label (input : Prims.string) (pos : Prims.nat) :
   Prims.nat Parser_Combinators.parse_result=
   let len = Parser_FastString.fs_byte_length input in
@@ -463,8 +540,8 @@ let count_nquads_quads (input : Prims.string) : Prims.nat=
   let len = Parser_FastString.fs_byte_length input in
   count_nquads_acc input Prims.int_zero Prims.int_zero (len + Prims.int_one)
 let rec parse_nquads_strict_acc (input : Prims.string) (pos : Prims.nat)
-  (ds : RDF_Graph_Executable.rdf_dataset) (fuel : Prims.nat) :
-  RDF_Graph_Executable.rdf_dataset FStar_Pervasives_Native.option=
+  (ds : RDF_Graph.rdf_dataset) (fuel : Prims.nat) :
+  RDF_Graph.rdf_dataset FStar_Pervasives_Native.option=
   if fuel = Prims.int_zero
   then FStar_Pervasives_Native.None
   else
@@ -523,23 +600,22 @@ let rec parse_nquads_strict_acc (input : Prims.string) (pos : Prims.nat)
                 | Parser_Combinators.ParseFail (uu___5, uu___6) ->
                     FStar_Pervasives_Native.None))))
 let parse_nquads_strict (input : Prims.string) :
-  RDF_Graph_Executable.rdf_dataset FStar_Pervasives_Native.option=
+  RDF_Graph.rdf_dataset FStar_Pervasives_Native.option=
   let len = Parser_FastString.fs_byte_length input in
-  match parse_nquads_strict_acc input Prims.int_zero
-          RDF_Graph_Executable.empty_dataset (len + Prims.int_one)
+  match parse_nquads_strict_acc input Prims.int_zero RDF_Graph.empty_dataset
+          (len + Prims.int_one)
   with
   | FStar_Pervasives_Native.Some ds ->
       FStar_Pervasives_Native.Some (RDF_Graph_Executable.dataset_finalise ds)
   | FStar_Pervasives_Native.None -> FStar_Pervasives_Native.None
 type nquad =
   {
-  nq_triple: RDF_Graph_Executable.triple ;
-  nq_graph: RDF_Graph_Executable.iri FStar_Pervasives_Native.option }
-let __proj__Mknquad__item__nq_triple (projectee : nquad) :
-  RDF_Graph_Executable.triple=
+  nq_triple: RDF_Triple.triple ;
+  nq_graph: RDF_Term.iri FStar_Pervasives_Native.option }
+let __proj__Mknquad__item__nq_triple (projectee : nquad) : RDF_Triple.triple=
   match projectee with | { nq_triple; nq_graph;_} -> nq_triple
 let __proj__Mknquad__item__nq_graph (projectee : nquad) :
-  RDF_Graph_Executable.iri FStar_Pervasives_Native.option=
+  RDF_Term.iri FStar_Pervasives_Native.option=
   match projectee with | { nq_triple; nq_graph;_} -> nq_graph
 let rec parse_nquads_flat_acc (input : Prims.string) (pos : Prims.nat)
   (acc : nquad Prims.list) (fuel : Prims.nat) : nquad Prims.list=
